prove req P in simple.lean

Computability/Simple.lean
@@ -5,7 +5,7 @@ import Mathlib.Data.Set.Finite.Basic
 
 open Computability
 open Computability.Code
-
+open List
 
 def PFun.nat_graph (f : ℕ→.ℕ) : Set ℕ := { xy | xy.unpair.2 ∈ f xy.unpair.1 }
 def total_graph (f : ℕ → ℕ) : Set ℕ := { xy | xy.unpair.2 = f xy.unpair.1 }
@@ -343,7 +343,7 @@ match s with
   -- }
   -- 0
 
-  List.foldr (step s) ⟪A,R⟫ (List.reverse $ List.range (s+1))
+  foldr (step s) ⟪A,R⟫ (range s).reverse
 
   -- if found : ∃ i ≤ s+1, ∃ x ∈ Wn ∅ i s, x > 2*i then
   --   let i := Nat.find found
@@ -393,17 +393,21 @@ theorem step_preserves_R_not_mem {j k s prev} (h:¬fs_in prev.r j) (hk:k<j) :
     next h_2 => simp_all only [gt_iff_lt, not_exists, not_and, not_lt]
   next h_1 => simp_all only [Bool.not_eq_false]
 
-theorem split_upper (h:fs_in R j) : fs_in (List.foldr (step s) ⟪A,R⟫ l).r j := by
+theorem fold_preserves_R_mem (h:fs_in R j) : fs_in (foldr (step s) ⟪A,R⟫ l).r j := by
   induction l with
   | nil => simpa
   | cons head tail ih => exact step_preserves_R_mem ih
+theorem fold_preserves_A_mem (h:fs_in A j) : fs_in (foldr (step s) ⟪A,R⟫ l).l j := by
+  induction l with
+  | nil => simpa
+  | cons head tail ih => exact step_preserves_A_mem ih
 
-theorem split_lower (h:¬fs_in R j) (hk : k ≤ j):
-¬ fs_in (List.foldr (step s) ⟪A,R⟫ (List.reverse $ List.range k)).r j := by
+theorem split_lower (h : ¬ fs_in R j) (hk : k ≤ j):
+¬ fs_in (foldr (step s) ⟪A,R⟫ (range k).reverse).r j := by
   induction k with
   | zero => simp at *; assumption
   | succ k ih =>
-    simp [listrwgen, -List.foldr_reverse]
+    simp [listrwgen, -foldr_reverse]
     have kk : k≤ j := by exact Nat.le_of_succ_le hk
     have kk2 : k< j := by exact hk
     have ih1 := ih kk; clear ih
@@ -413,39 +417,179 @@ theorem split_lower (h:¬fs_in R j) (hk : k ≤ j):
     simp
     exact this
 
-theorem split_middle (h:¬fs_in R j) (h2: ∃ x ∈ Wn ∅ j s, x > 2*j) :
+theorem split_middle_R (h:¬fs_in R j) (h2: ∃ x ∈ Wn ∅ j s, x > 2*j) :
 fs_in ((step s) j ⟪A,R⟫).r j := by
   simp at h2
   simp [step, h, h2]
 
-theorem R_foldr (h:¬fs_in R j) (h2: ∃ x ∈ Wn ∅ j s, x > 2*j) (hs:j<s):
-fs_in (List.foldr (step s) ⟪A,R⟫ (List.reverse $ List.range (s+1))).r j := by
-  have : (List.reverse $ List.range (s+1)) = (List.range' (j+1) (s-j)).reverse ++ [j] ++ (List.range' 0 j).reverse := by
-    simp
-    have : j :: List.range' (j + 1) (s - j) = List.range' (0+j) (s - j +1) := by aesop
-    rw [this]
-    have : List.range (s + 1) = List.range' 0 (s + 1) := by exact List.range_eq_range'
-    rw [this]
-    have := @List.range'_append_1 0 j (s-j+1)
-    rw [this]
-    congr 1
-    grind
-  rw [this]
-  simp [-List.foldr_reverse]
+theorem split_middle_A {j:ℕ}
+  (h: ¬ (∃ x ∈ Wn ∅ j s, fs_in A x))
+  (h2: ∃ x ∈ Wn ∅ j s, x > 2*j)
+  (hj:¬fs_in R j) -- this is where interaction w A and R comes in the proof
+  :
+  -- ∃ x ∈ Wn ∅ j s, fs_in ((step s) j ⟪A,R⟫).l x := by
+  fs_in ((step s) j ⟪A,R⟫).l (Nat.find h2) := by
+  simp at h2
+  simp [step, h2]
 
-  rw [show List.range' 0 j = List.range j from by exact Eq.symm List.range_eq_range'] at *
-  let fold_lower := (List.foldr (step s) ⟪A,R⟫ (List.range j).reverse)
+  let x := Nat.find h2
+  let ⟨hx0, hx1⟩ := Nat.find_spec h2
+  -- use x
+  aesop
+
+theorem range_3way_split {s j} (hs:j<s) : (range (s+1)).reverse = (range' (j+1) (s-j)).reverse ++ [j] ++ (range' 0 j).reverse := by
+  simp
+  have : j :: range' (j + 1) (s - j) = range' (0+j) (s - j +1) := by aesop
+  rw [this]
+  have : range (s + 1) = range' 0 (s + 1) := by exact range_eq_range'
+  rw [this]
+  have := @range'_append_1 0 j (s-j+1)
+  rw [this]
+  congr 1
+  grind
+theorem range_3way_split2 {s j} (hs:j+1<s) : (range s).reverse = (range' (j+1) (s-1-j)).reverse ++ [j] ++ (range' 0 j).reverse := by
+  simp
+  have : j :: range' (j + 1) (s-1 - j) = range' (0+j) (s-1 - j +1) := by aesop
+  rw [this]
+  have : range (s) = range' 0 s := by exact range_eq_range'
+  rw [this]
+  have := @range'_append_1 0 j (s-1-j+1)
+  rw [this]
+  congr 1
+  grind
+
+theorem R_foldr (h:¬fs_in R j) (h2: ∃ x ∈ Wn ∅ j s, x > 2*j) (hs:j+1<s):
+fs_in (foldr (step s) ⟪A,R⟫ (range s).reverse).r j := by
+  rw [range_3way_split2 hs]
+  simp [-foldr_reverse]
+
+  rw [show range' 0 j = range j from by exact Eq.symm range_eq_range'] at *
+  let fold_lower := (foldr (step s) ⟪A,R⟫ (range j).reverse)
 
   have a0 := @split_lower R j j s A h (Nat.le_refl j)
-  rw [show  (List.foldr (step s) ⟪A,R⟫ (List.range j).reverse) = fold_lower from rfl] at ⊢ a0
-  have a1 := @split_middle _ j s (fold_lower.l) a0 h2
+  rw [show  (foldr (step s) ⟪A,R⟫ (range j).reverse) = fold_lower from rfl] at ⊢ a0
+  have a1 := @split_middle_R _ j s (fold_lower.l) a0 h2
   simp at a1
 
-  have a2 := @split_upper _ _  s ((step s j fold_lower).l) ((List.range' (j + 1) (s - j)).reverse) a1
+  have a2 := @fold_preserves_R_mem _ _  s (step s j fold_lower).l ((range' (j + 1) (s-1-j)).reverse) a1
 
-  simp at a2
-  simp
+  simp only [pair_lr] at a2
+  -- simp only []
   exact a2
+
+
+/-- R implies A -/
+def RiA (R A s : ℕ) := ∀ j, fs_in R j → ∃ x ∈ Wn ∅ (n2c j) s, fs_in A x
+theorem R_imp_A_prop_step (R A s : ℕ) : RiA R A s → ∀ k, RiA (step s k ⟪A,R⟫).r (step s k ⟪A,R⟫).l s := by
+  simp [RiA]
+  simp [step]
+
+  -- proved by doing aesop?, then manually resolving dangling cases
+  intro h0
+  intro k j a
+  split
+  next h =>
+    simp_all only [↓reduceIte, gt_iff_lt]
+    split
+    next h_1 =>
+      simp_all only [gt_iff_lt, ↓reduceDIte, pair_r, Nat.testBit_or, Bool.or_eq_true, pair_l]
+      -- obtain ⟨w, h_1⟩ := h_1
+      -- obtain ⟨left, right⟩ := h_1
+      cases a with
+      | inl h_3 =>
+        exact (h0 j h_3).elim λ x hx ↦ ⟨x, @evaln_mono_dom (χ ∅) s s j x (Nat.le_refl s) hx.1, Or.inl hx.2⟩
+      | inr h_2 =>
+        have kj : k=j := by contrapose h_2; simp [h_2]
+        let x := Nat.find h_1
+        let hx := Nat.find_spec h_1
+        rw [show Nat.find h_1 = x from rfl] at hx ⊢
+        simp [kj] at hx ⊢
+        use x
+        constructor
+        exact @evaln_mono_dom (χ ∅) s s j x (Nat.le_refl s) (hx.1)
+        simp only [Nat.testBit_two_pow_self, or_true]
+    next h_1 =>
+      simp_all only [gt_iff_lt, ↓reduceDIte, pair_r, not_exists, not_and, not_lt, pair_l]
+      -- exact (h0 j a).elim λ x hx ↦ ⟨x, @evaln_mono_dom (χ ∅) s s j x (Nat.le_refl s) hx.1, hx.2⟩
+  next h =>
+    simp_all only [Bool.true_eq_false, ↓reduceIte, pair_r, Bool.not_eq_false, pair_l]
+    -- exact (h0 j a).elim λ x hx ↦ ⟨x, @evaln_mono_dom (χ ∅) s s j x (Nat.le_refl s) hx.1, hx.2⟩
+
+theorem RiA_foldr
+-- foldr (step s) ⟪A,R⟫ (range j).reverse
+  -- (hbase : ¬∃ x ∈ Wn ∅ (n2c j) s, fs_in A x)
+  -- (hj:fs_in (foldr (step s) ⟪A,R⟫ (range j).reverse).r j) :
+  -- ∃ x ∈ Wn ∅ (n2c j) s, fs_in (foldr (step s) ⟪A,R⟫ (range j).reverse).l x = true := by sorry
+  : RiA R A s → ∀ j, RiA (foldr (step s) ⟪A,R⟫ (range j).reverse).r (foldr (step s) ⟪A,R⟫ (range j).reverse).l s := by
+    intro h
+    intro j
+    induction j with
+    | zero => simpa
+    | succ j ih =>
+      simp [listrwgen, -foldr_reverse]
+      have := R_imp_A_prop_step _ _ s ih j
+      simp only [pair_lr] at this
+      exact this
+
+theorem RiA_C : ∀ s, RiA (C s).r (C s).l s := by
+  intro s
+  induction s with
+  | zero => simp [C, RiA]
+  | succ s ih =>
+    simp [C, RiA, -foldr_reverse]
+    intro j h
+    have := @RiA_foldr (C s).r (C s).l s ih s j
+    simp only [pair_lr] at this
+    have := this h
+    rcases this with ⟨x,hx0,hx1⟩
+    use x
+    constructor
+    simp at hx0
+    exact @evalnSet_mono_dom ∅ s (s+1) j x (Nat.le_add_right s 1) hx0
+    exact hx1
+
+
+theorem A_foldr {j s : ℕ}
+  (h  : ¬ (∃ x ∈ Wn ∅ j s, fs_in A x))
+  (h2 : ∃ x ∈ Wn ∅ j s, x > 2*j)
+  (hs : j<s) :
+  (∃ x ∈ Wn ∅ j s, fs_in (foldr (step s) ⟪A,R⟫ (range (s+1)).reverse).l x) := by
+
+  rw [range_3way_split hs]
+  simp [-foldr_reverse]
+
+  rw [show range' 0 j = range j from by exact Eq.symm range_eq_range'] at *
+  let fold_lower := (foldr (step s) ⟪A,R⟫ (range j).reverse)
+  rw [show  (foldr (step s) ⟪A,R⟫ (range j).reverse) = fold_lower from rfl] at ⊢
+  -- by_cases h3:fs_in fold_lower.l x
+  by_cases h3:(∃ x ∈ Wn ∅ j s, fs_in fold_lower.l x)
+  ·
+    obtain ⟨x,hx0,hx1⟩ := h3
+    use x
+    have a0 := @step_preserves_A_mem x s j fold_lower hx1
+    have a1 := @fold_preserves_A_mem _ _ s (step s j fold_lower).r (range' (j + 1) (s - j)).reverse a0
+    simp at a1
+    simp
+    exact ⟨hx0, a1⟩
+  ·
+    let x := Nat.find h2
+    let ⟨hx0, hx1⟩ := Nat.find_spec h2
+    use x
+
+    constructor
+    exact hx0
+
+    have a0 := @split_middle_A _ _ fold_lower.r _ h3 h2 ?_
+    simp at a0
+    -- rcases a0 with ⟨a2,a3,a4⟩
+
+    have a1 := @fold_preserves_A_mem _ _ s (step s j fold_lower).r (range' (j + 1) (s - j)).reverse a0
+
+    simp [-foldr_reverse] at a1
+    exact a1
+
+
+    sorry
 
 
 def A : Set ℕ := {x | ∃ s, fs_in (C s).l x}
@@ -483,22 +627,48 @@ theorem P (i:ℕ) : (W ∅ i).Infinite → (∃ s, fs_in (C s).r i ∧ ∃ y ∈
 
   rcases this with ⟨x, hx0, hx1⟩
   rcases Wn_complete.mp hx0 with ⟨s,hs⟩
-  have si1 : s ≤ s+i+1 := by omega
-  have si2 : i < s+i+1 := by omega
-  have ex0 :  ∃ x ∈ Wn ∅ (n2c i) (s+i+1), x > 2 * i := by
+  have si1 : s ≤ s+i+2 := by omega
+  have si2 : i+1 < s+i+2 := by omega
+  have ex0 :  ∃ x ∈ Wn ∅ (n2c i) (s+i+2), x > 2 * i := by
     exact ⟨x,Wn_mono (si1) hs, hx1⟩
-  use s+i+1+1
+  use s+i+2+1
+  -- constructor
   unfold C
-  constructor
   -- cases fs in prev R
   lift_lets; extract_lets; expose_names
   by_cases h1:fs_in R i
   ·
-    exact split_upper h1
-  ·
-    have := @R_foldr _ _ _ A h1 ex0 si2
-    exact this
+    have a0 := @fold_preserves_R_mem R i (s+i+2) A (range (s + i + 2)).reverse h1
+    constructor
+    exact a0
 
+    have := @RiA_foldr R A (s+i+2) ?_ (s+i+2)
+    unfold RiA at this
+    have := this i a0
+    rcases this with ⟨w,hw0,hw1⟩
+    use w
+    constructor
+    exact Wn_sound hw0
+    exact hw1
+    exact RiA_C (s + i + 2)
+
+    -- exact @fold_preserves_R_mem R i (s+i+2) A (range (s + i + 2)).reverse h1
+    -- exact fold_preserves_R_mem h1
+  ·
+    have a0 := @R_foldr _ _ _ A h1 ex0 si2
+    constructor
+    exact a0
+    
+
+    have := @RiA_foldr R A (s+i+2) ?_ (s+i+2)
+    unfold RiA at this
+    have := this i  a0
+    rcases this with ⟨w,hw0,hw1⟩
+    use w
+    constructor
+    exact Wn_sound hw0
+    exact hw1
+    exact RiA_C (s + i + 2)
 
 
 --   have main : ∃ y, fs_in (C (s+i)).l y ∧ y ∈ W O i := by
@@ -511,7 +681,7 @@ theorem P (i:ℕ) : (W ∅ i).Infinite → (∃ s, fs_in (C s).r i ∧ ∃ y ∈
 --   -- unfold A
 
 --   -- have : ¬ fs_in R i := by sorry
-  sorry
+  
 theorem N (i:ℕ) : (W O i).Infinite → (W O i ∩ W O a ≠ ∅) := by
   sorry
 
